Introduce [flag] type to be a refinement on integers. Introduce aliases for carry and overflow flags.

vale/specs/hardware/Vale.X64.Machine_s.fst
@@ -11,9 +11,13 @@ let int_to_nat64 (i:int) : n:nat64{0 <= i && i < pow2_64 ==> i == n} =
 unfold let nat128 = Vale.Def.Words_s.nat128
 unfold let quad32 = Vale.Def.Types_s.quad32
 
+type flag:eqtype = i:int{0 <= i /\ i < 16}
 type reg:eqtype = i:int{0 <= i /\ i < 16}
 type xmm:eqtype = i:int{0 <= i /\ i < 16}
 type imm8:eqtype = i:int{0 <= i && i < 256}
+
+[@va_qattr] unfold let fCarry    : flag = 0
+[@va_qattr] unfold let fOverflow : flag = 11
 
 [@va_qattr] unfold let rRax : reg = 0
 [@va_qattr] unfold let rRbx : reg = 1
